code/experimental/P256/Hacl.Impl.P256.fsti
@@ -102,6 +102,36 @@ val point_double: p: point -> result: point -> tempBuffer: lbuffer uint64 (size 
 
 
 
+val point_add: p: point -> q: point -> result: point -> tempBuffer: lbuffer uint64 (size 88) -> 
+   Stack unit (requires fun h -> live h p /\ live h q /\ live h result /\ live h tempBuffer /\ 
+   eq_or_disjoint q result /\
+   disjoint p q /\ disjoint p tempBuffer /\ disjoint q tempBuffer /\ disjoint p result /\ disjoint result tempBuffer /\  
+    as_nat h (gsub p (size 8) (size 4)) < prime /\ 
+    as_nat h (gsub p (size 0) (size 4)) < prime /\ 
+    as_nat h (gsub p (size 4) (size 4)) < prime /\
+    as_nat h (gsub q (size 8) (size 4)) < prime /\ 
+    as_nat h (gsub q (size 0) (size 4)) < prime /\  
+    as_nat h (gsub q (size 4) (size 4)) < prime 
+    ) 
+   (ensures fun h0 _ h1 -> 
+     modifies (loc tempBuffer |+| loc result) h0 h1 /\ 
+     as_nat h1 (gsub result (size 8) (size 4)) < prime /\ 
+     as_nat h1 (gsub result (size 0) (size 4)) < prime /\ 
+     as_nat h1 (gsub result (size 4) (size 4)) < prime /\
+     (
+       let pX, pY, pZ = gsub p (size 0) (size 4), gsub p (size 4) (size 4), gsub p (size 8) (size 4) in 
+       let qX, qY, qZ = gsub q (size 0) (size 4), gsub q (size 4) (size 4), gsub q (size 8) (size 4) in 
+       let x3, y3, z3 = gsub result (size 0) (size 4), gsub result (size 4) (size 4), gsub result (size 8) (size 4) in 
+       
+       let pxD, pyD, pzD = fromDomain_ (as_nat h0 pX), fromDomain_ (as_nat h0 pY), fromDomain_ (as_nat h0 pZ) in 
+       let qxD, qyD, qzD = fromDomain_ (as_nat h0 qX), fromDomain_ (as_nat h0 qY), fromDomain_ (as_nat h0 qZ) in 
+       let x3D, y3D, z3D = fromDomain_ (as_nat h1 x3), fromDomain_ (as_nat h1 y3), fromDomain_ (as_nat h1 z3) in
+      
+       let xN, yN, zN = _point_add (pxD, pyD, pzD) (qxD, qyD, qzD) in 
+       x3D == xN /\ y3D == yN /\ z3D == zN
+  )
+)
+
 val isPointAtInfinityPrivate: p: point -> Stack uint64
   (requires fun h -> live h p /\ as_nat h (gsub p (size 8) (size 4)) < prime)
   (ensures fun h0 r h1 -> modifies0 h0 h1 /\          
